lean/AbsDen.lean
@@ -1,5 +1,8 @@
 import AbsDen.Syntax
-import AbsDen.ToposOfTrees
+import AbsDen.World
+import AbsDen.World.DeriveTests
 import AbsDen.Env
 import AbsDen.Semantics
-import AbsDen.Concrete
+import AbsDen.Trace
+import AbsDen.ByName
+import AbsDen.ByNeed
